Foundation/ProvabilityLogic/S/Completeness.lean
@@ -1,156 +1,16 @@
 import Foundation.Modal.Logic.Extension
+import Foundation.Modal.Logic.S
+import Foundation.Modal.Kripke.ExtendRoot2
 import Foundation.ProvabilityLogic.GL.Completeness
+import Foundation.Modal.Boxdot.Basic
 import Mathlib.Tactic.TFAE
 
-namespace LO
 
-namespace Modal
-
-section
-
-variable {M : Kripke.Model} {x : M.World} {φ ψ : Formula ℕ} {Γ : FormulaFinset ℕ}
-
-lemma Formula.Kripke.Satisfies.finset_conj_def : x ⊧ Γ.conj ↔ ∀ φ ∈ Γ, x ⊧ φ := by
-  simp only [Semantics.realize_finset_conj, Satisfies.iff_models];
-
-end
-
-section
-
-open Logic
-
-protected abbrev Logic.S := addQuasiNormal Logic.GL (Axioms.T (.atom 0))
-instance : Logic.S.QuasiNormal where
-  subset_K := by
-    intro φ hφ;
-    apply Logic.sumQuasiNormal.mem₁;
-    exact Logic.of_mem_K hφ;
-  mdp_closed := by
-    intro φ ψ hφψ hφ;
-    apply Logic.sumQuasiNormal.mdp hφψ hφ;
-  subst_closed := by
-    intro φ hφ s;
-    apply Logic.sumQuasiNormal.subst;
-    exact hφ;
-
-lemma Logic.S.mem_axiomT : □φ ➝ φ ∈ Logic.S := by
-  apply Logic.subst (φ := Axioms.T (.atom 0)) (s := λ _ => φ);
-  apply Logic.sumQuasiNormal.mem₂;
-  tauto;
-
-lemma GL_subset_S : Logic.GL ⊆ Logic.S := by
-  intro φ hφ;
-  apply Logic.sumQuasiNormal.mem₁;
-  assumption;
-
-private inductive Logic.S' : Logic
-  | mem_GL {φ} : φ ∈ Logic.GL → Logic.S' φ
-  | axiomT (φ) : Logic.S' (Axioms.T φ)
-  | mdp  {φ ψ} : Logic.S' (φ ➝ ψ) → Logic.S' φ → Logic.S' ψ
-
-private lemma Logic.eq_S_S' : Logic.S = Logic.S' := by
-  ext φ;
-  constructor;
-  . intro h;
-    induction h with
-    | mem₁ h => exact Logic.S'.mem_GL h;
-    | mem₂ h => subst h; exact Logic.S'.axiomT (.atom 0);
-    | mdp _ _ ihφψ ihφ => exact Logic.S'.mdp ihφψ ihφ;
-    | subst hφ ihφ =>
-      clear hφ;
-      induction ihφ with
-      | mem_GL h =>
-        apply Logic.S'.mem_GL;
-        exact Logic.subst h;
-      | axiomT _ => apply Logic.S'.axiomT;
-      | mdp _ _ ihφψ ihφ =>
-        apply Logic.S'.mdp ihφψ ihφ;
-  . intro h;
-    induction h with
-    | mem_GL h => exact sumQuasiNormal.mem₁ h;
-    | mdp _ _ ihφψ ihφ => exact sumQuasiNormal.mdp ihφψ ihφ;
-    | axiomT φ =>
-      exact sumQuasiNormal.subst (φ := Axioms.T (.atom 0)) (s := λ _ => φ) $ by
-        apply Logic.sumQuasiNormal.mem₂;
-        simp;
-
--- TODO: Remove `eq_S_S'`?
-protected def Logic.S.rec'
-  {motive : (φ : Formula ℕ) → φ ∈ Logic.S → Prop}
-  (mem_GL : ∀ {φ}, (h : φ ∈ Logic.GL) → motive φ (sumQuasiNormal.mem₁ h))
-  (axiomT : ∀ {φ}, motive (Axioms.T φ) (sumQuasiNormal.subst (φ := Axioms.T (.atom 0)) (s := λ _ => φ) (sumQuasiNormal.mem₂ (by tauto))))
-  (mdp : ∀ {φ ψ}, {hφψ : φ ➝ ψ ∈ Logic.S} → {hφ : φ ∈ Logic.S} → (motive (φ ➝ ψ) hφψ) → (motive φ hφ) → motive ψ (sumQuasiNormal.mdp hφψ hφ))
-  : ∀ {φ}, (h : φ ∈ Logic.S) → motive φ h := by
-  intro φ h;
-  rw [Logic.eq_S_S'] at h;
-  induction h with
-  | mem_GL h => apply mem_GL; assumption;
-  | axiomT h => exact axiomT;
-  | mdp hφψ hφ ihφψ ihφ =>
-    apply mdp;
-    . apply ihφψ;
-    . apply ihφ;
-    . rwa [←Logic.eq_S_S'] at hφψ;
-    . rwa [←Logic.eq_S_S'] at hφ;
+noncomputable abbrev LO.Modal.Formula.rflSubformula [DecidableEq α] (φ : Formula α) : FormulaFinset α
+  := (φ.subformulas.prebox.image (λ ψ => □ψ ➝ ψ))
 
 
-namespace Logic
-
-open Entailment
-
-variable {L : Modal.Logic} [L.QuasiNormal] {φ ψ : Formula ℕ}
-
-lemma p_q_Apq (hφ : φ ∈ L) (hψ : ψ ∈ L) : φ ⋏ ψ ∈ L := by
-  apply Logic.mdp (φ := ψ);
-  apply Logic.mdp (φ := φ) (ψ := ψ ➝ φ ⋏ ψ);
-  . apply Logic.of_mem_K;
-    exact and₃!;
-  . assumption;
-  . assumption;
-
-lemma conj_iffAux {Γ : List (Formula ℕ)} : Γ.conj₂ ∈ L ↔ ∀ φ ∈ Γ, φ ∈ L := by
-  constructor;
-  . intro h φ hφ;
-    refine Logic.mdp ?_ h;
-    apply Logic.of_mem_K;
-    apply general_conj'! hφ;
-  . intro h;
-    induction Γ using List.induction_with_singleton with
-    | hnil =>
-      simp only [List.conj₂_nil];
-      apply Logic.of_mem_K;
-      exact verum!;
-    | hsingle φ =>
-      apply h;
-      simp;
-    | @hcons φ Γ hΓ ih =>
-      simp [List.conj₂_cons_nonempty hΓ];
-      apply p_q_Apq;
-      . apply h; tauto;
-      . apply ih; tauto;
-
-lemma conj_iff {Γ : FormulaFinset ℕ} : Γ.conj ∈ L ↔ ∀ φ ∈ Γ, φ ∈ L := by
-  constructor;
-  . intro h φ hφ;
-    apply Logic.conj_iffAux (Γ := Γ.toList) |>.mp $ h;
-    simpa;
-  . intro h;
-    apply Logic.conj_iffAux (Γ := Γ.toList) |>.mpr;
-    intro φ hφ;
-    apply h;
-    simpa using hφ;
-
-end Logic
-
-end
-
-variable {α} [DecidableEq α]
-
-noncomputable abbrev Formula.rflSubformula (φ : Formula α) : FormulaFinset α := (φ.subformulas.prebox.image (λ ψ => □ψ ➝ ψ))
-
-end Modal
-
-namespace ProvabilityLogic
+namespace LO.ProvabilityLogic
 
 open Entailment
 open Modal
@@ -213,7 +73,7 @@ lemma GL_S_TFAE :
   ].TFAE := by
   tfae_have 1 → 2 := by
     intro h;
-    apply Logic.S.mdp (GL_subset_S h) ?_;
+    apply Logic.S.mdp (Logic.GL_subset_S h) ?_;
     apply Logic.conj_iff.mpr;
     suffices ∀ B, □B ∈ A.subformulas → □B ➝ B ∈ Logic.S by simpa [Formula.rflSubformula];
     rintro B _;
@@ -329,10 +189,65 @@ lemma GL_S_TFAE :
 
 theorem S.arithmetical_completeness_iff : A ∈ Logic.S ↔ ∀ f : Realization ℒₒᵣ, ℕ ⊧ₘ₀ (f.interpret ((𝐈𝚺₁).standardDP T) A) := GL_S_TFAE.out 1 2
 
-lemma _root_.LO.Modal.Logic.iff_provable_rfl_GL_provable_S : (A.rflSubformula.conj ➝ A) ∈ Logic.GL ↔ A ∈ Logic.S := GL_S_TFAE (T := 𝐈𝚺₁) |>.out 0 1
-
 end
 
 end ProvabilityLogic
+
+
+
+namespace Modal.Logic
+
+open Kripke Formula.Kripke
+
+variable {A : Formula _}
+
+lemma iff_provable_rflSubformula_GL_provable_S : (A.rflSubformula.conj ➝ A) ∈ Logic.GL ↔ A ∈ Logic.S := ProvabilityLogic.GL_S_TFAE (T := 𝐈𝚺₁) |>.out 0 1
+
+lemma iff_provable_boxdot_GL_provable_boxdot_S : Aᵇ ∈ Logic.GL ↔ Aᵇ ∈ Logic.S := by
+  constructor;
+  . apply Logic.GL_subset_S;
+  . intro h;
+    replace h := iff_provable_rflSubformula_GL_provable_S.mpr h;
+    replace h := Hilbert.GL.Kripke.iff_provable_satisfies_FiniteTransitiveTree.mp h;
+    apply Hilbert.GL.Kripke.iff_provable_satisfies_FiniteTransitiveTree.mpr;
+    intro M r _;
+    obtain ⟨i, hi⟩ := Kripke.Model.extendRoot₂.inr_satisfies_axiomT_set (M := M) (Γ := Aᵇ.subformulas.prebox)
+    let M₁ := M.extendRoot₂ r ⟨Aᵇ.subformulas.prebox.card + 1, by omega⟩;
+    let i₁ : M₁.World := Sum.inl i;
+    refine Model.extendRoot₂.inl_satisfies_boxdot_iff.mpr
+      $ Model.pointGenerate.modal_equivalent_at_root (r := i₁) |>.mp
+      $ @h (M₁↾i₁) Model.pointGenerate.root ?_ ?_;
+    . apply Frame.isFiniteTree_iff _ _ |>.mpr
+      constructor;
+      . apply Frame.pointGenerate.isFinite (finite := Frame.extendRoot₂.isFinite)
+      . apply Frame.isTree_iff _ _ |>.mpr;
+        refine ⟨?_, ?_, ?_⟩;
+        . apply Frame.pointGenerate.instIsRooted;
+        . apply Frame.pointGenerate.isAsymm (assym := Frame.extendRoot₂.isAsymm);
+        . apply Frame.pointGenerate.isTrans (trans := Frame.extendRoot₂.isTrans);
+    . apply @Model.pointGenerate.modal_equivalent_at_root (r := i₁) |>.mpr
+      apply Satisfies.finset_conj_def.mpr;
+      intro B hB;
+      apply Satisfies.finset_conj_def.mp hi;
+      simp only [Finset.mem_image, Finset.eq_prebox_premultibox_one, Finset.mem_preimage, Function.iterate_one] at hB ⊢;
+      obtain ⟨C, hC, rfl⟩ := hB;
+      use C;
+
+theorem S.no_bot : ⊥ ∉ Logic.S := by
+  have hb : (⊥ : Formula ℕ) = ⊥ᵇ := by simp [Formula.BoxdotTranslation];
+  rw [hb];
+  apply iff_provable_boxdot_GL_provable_boxdot_S.not.mp;
+  rw [←hb];
+  apply Logic.no_bot;
+
+instance : Logic.S.Consistent := ⟨by
+  apply Set.eq_univ_iff_forall.not.mpr;
+  push_neg;
+  use ⊥;
+  exact Logic.S.no_bot;
+⟩
+
+end Modal.Logic
+
 
 end LO
