Foundation/Modal/Logic/S.lean
@@ -1,0 +1,98 @@
+import Foundation.Modal.Logic.Extension
+import Foundation.ProvabilityLogic.GL.Completeness
+
+namespace LO.Modal
+
+open Logic
+
+protected abbrev Logic.S := addQuasiNormal Logic.GL (Axioms.T (.atom 0))
+instance : Logic.S.QuasiNormal where
+  subset_K := by
+    intro φ hφ;
+    apply Logic.sumQuasiNormal.mem₁;
+    exact Logic.of_mem_K hφ;
+  mdp_closed := by
+    intro φ ψ hφψ hφ;
+    apply Logic.sumQuasiNormal.mdp hφψ hφ;
+  subst_closed := by
+    intro φ hφ s;
+    apply Logic.sumQuasiNormal.subst;
+    exact hφ;
+
+lemma Logic.S.mem_axiomT : □φ ➝ φ ∈ Logic.S := by
+  apply Logic.subst (φ := Axioms.T (.atom 0)) (s := λ _ => φ);
+  apply Logic.sumQuasiNormal.mem₂;
+  tauto;
+
+
+lemma Logic.GL_subset_S : Logic.GL ⊆ Logic.S := by
+  intro φ hφ;
+  apply Logic.sumQuasiNormal.mem₁;
+  assumption;
+
+lemma Logic.GL_ssubset_S : Logic.GL ⊂ Logic.S := by
+  constructor;
+  . exact Logic.GL_subset_S;
+  . suffices ∃ φ, φ ∈ Logic.S ∧ φ ∉ Logic.GL by exact Set.not_subset.mpr this;
+    use (Axioms.T (.atom 0));
+    constructor;
+    . exact Logic.S.mem_axiomT;
+    . exact Hilbert.GL.unprovable_AxiomT;
+instance : ProperSublogic Logic.GL Logic.S := ⟨Logic.GL_ssubset_S⟩
+
+
+section
+
+private inductive Logic.S' : Logic
+  | mem_GL {φ} : φ ∈ Logic.GL → Logic.S' φ
+  | axiomT (φ) : Logic.S' (Axioms.T φ)
+  | mdp  {φ ψ} : Logic.S' (φ ➝ ψ) → Logic.S' φ → Logic.S' ψ
+
+private lemma Logic.eq_S_S' : Logic.S = Logic.S' := by
+  ext φ;
+  constructor;
+  . intro h;
+    induction h with
+    | mem₁ h => exact Logic.S'.mem_GL h;
+    | mem₂ h => subst h; exact Logic.S'.axiomT (.atom 0);
+    | mdp _ _ ihφψ ihφ => exact Logic.S'.mdp ihφψ ihφ;
+    | subst hφ ihφ =>
+      clear hφ;
+      induction ihφ with
+      | mem_GL h =>
+        apply Logic.S'.mem_GL;
+        exact Logic.subst h;
+      | axiomT _ => apply Logic.S'.axiomT;
+      | mdp _ _ ihφψ ihφ =>
+        apply Logic.S'.mdp ihφψ ihφ;
+  . intro h;
+    induction h with
+    | mem_GL h => exact sumQuasiNormal.mem₁ h;
+    | mdp _ _ ihφψ ihφ => exact sumQuasiNormal.mdp ihφψ ihφ;
+    | axiomT φ =>
+      exact sumQuasiNormal.subst (φ := Axioms.T (.atom 0)) (s := λ _ => φ) $ by
+        apply Logic.sumQuasiNormal.mem₂;
+        simp;
+
+-- TODO: Remove `eq_S_S'`?
+protected def Logic.S.rec'
+  {motive : (φ : Formula ℕ) → φ ∈ Logic.S → Prop}
+  (mem_GL : ∀ {φ}, (h : φ ∈ Logic.GL) → motive φ (sumQuasiNormal.mem₁ h))
+  (axiomT : ∀ {φ}, motive (Axioms.T φ) (sumQuasiNormal.subst (φ := Axioms.T (.atom 0)) (s := λ _ => φ) (sumQuasiNormal.mem₂ (by tauto))))
+  (mdp : ∀ {φ ψ}, {hφψ : φ ➝ ψ ∈ Logic.S} → {hφ : φ ∈ Logic.S} → (motive (φ ➝ ψ) hφψ) → (motive φ hφ) → motive ψ (sumQuasiNormal.mdp hφψ hφ))
+  : ∀ {φ}, (h : φ ∈ Logic.S) → motive φ h := by
+  intro φ h;
+  rw [Logic.eq_S_S'] at h;
+  induction h with
+  | mem_GL h => apply mem_GL; assumption;
+  | axiomT h => exact axiomT;
+  | mdp hφψ hφ ihφψ ihφ =>
+    apply mdp;
+    . apply ihφψ;
+    . apply ihφ;
+    . rwa [←Logic.eq_S_S'] at hφψ;
+    . rwa [←Logic.eq_S_S'] at hφ;
+
+end
+
+end LO.Modal
